$e'=e\cdot e'=e$ ^NeutralIsUnique

Suppose there are two inverses $h,h'$, then $h=h(gh')=hgh'=(hg)h'=h'$ 
^InverseIsUnique

$g\cdot g^{-1}=g^{-1}\cdot g=e$, then by the definition of inverse, the inverse of $g^{-1}$ is $g$, which inplies $g=(g^{-1})^{-1}$ ^InverseOfInverse

$(h^{-1}\circ g^{-1})\circ (gh)=h^{-1}\circ g^{-1}\circ g\circ h=e$, the inverse is also true ^InverseOfProduct

1). $1\in H_{i}$ for arbitrary $i\in I\ \Longrightarrow 1\in \bigcap_{i\in I}H_{i}$
2). if $x,y\in \bigcap_{i\in I}H_{i},\ x,y\in H_{i}$ for arbitrary $i$, $xy\in H_{i}$ for arbitrary $i$ $\Longrightarrow \ xy\in \bigcap_{i\in I}H_{i}$   ^9ce490

"$\Longleftarrow$" Obvious
"$\Longrightarrow$" $A\subseteq H,\ <A>=\bigcap_{K\leq G,A\subseteq K}K$, but $H$ is one of the $K$, so according to [[001 Group#^RemarkOne|Remark]], $<A>\leq H$  ^89ccb6
